prove forward rules of a cryptid

BusyLean/BB62.lean
@@ -36,3 +36,19 @@ notation3 l " {{F}}> " r => (F, (⟨ListBlank.head r, l, ListBlank.tail r⟩ : T
 
 notation3 "Side" => ListBlank Symbol
 notation3 "TM62" => @TM State Symbol
+
+@[simp]
+def list_nat_repeat (l : List α) (n : Nat) := match n with
+  | 0 => []
+  | n + 1 => List.append l (list_nat_repeat l n)
+
+instance instHPowListNat : HPow (List Symbol) Nat (List Symbol) := ⟨list_nat_repeat⟩
+
+theorem list_pow_add (l : List Symbol) (n m : Nat) : l^(n + m) = l^n ++ l^m := match m with
+  | 0 => by
+    simp_rw [HPow.hPow, add_zero, list_nat_repeat, List.append_nil]
+  | m + 1 => by
+    rw [add_comm m 1, ← add_assoc, add_comm 1 m, list_pow_add]
+    simp only [HPow.hPow, list_nat_repeat, List.append_eq, List.append_assoc]
+    rw [← List.append_assoc, ← List.append_assoc, List.append_cancel_right_eq]
+    induction' n with n ih <;> [simp; simpa]
